dafny/top-down/top-down2.dfy
@@ -50,6 +50,17 @@ method find_matching_rules(rules: seq<Rule>, goal:SearchClause) returns (c:seq<R
     return matching_rules;
 }
 
+/*
+RuleHead: A(P, P) :- something
+Goal : A(X, Y)
+goal.subst : X-->ev1, Y-->ev2
+
+unify(RuleHead, Goal) : P-->ev1
+
+we want: X-->P, Y-->P (because we map the P in subst to whatever evar X points to)
+
+therefore if forall P,Q, they are resolved to consts, then X,Y also have to
+*/
 
 method unify(head_clause:Clause, goal:SearchClause, emap:EvarMap) returns (o:Option<EvarSubstitution>)//, e:EvarMap)
     requires emap.inv()
@@ -57,6 +68,7 @@ method unify(head_clause:Clause, goal:SearchClause, emap:EvarMap) returns (o:Opt
     requires |head_clause.terms| == |goal.evar_terms|
     requires goal.valid()
     requires goal.valid_emap(emap)
+    requires goal.name == head_clause.name
     modifies emap
     ensures emap.is_more_resolved()
     ensures goal.valid_emap(emap)
@@ -66,12 +78,20 @@ method unify(head_clause:Clause, goal:SearchClause, emap:EvarMap) returns (o:Opt
     ensures o.Some? ==> forall e :: o.value.in2(e) ==> e in emap.evar_map
     // ensures o.Some? ==> forall v :: v in goal.clause.terms && v.Var? ==> o.value.in1(v) // IS WRONG
     ensures o.Some? ==> forall v :: v in head_clause.terms && v.Var? ==> o.value.in1(v)
-    ensures head_clause.is_ground() && o.Some? ==> goal.emap_fully_resolved(emap)
+    ensures o.Some? ==> forall i:nat | i < |head_clause.terms| && head_clause.terms[i].Var? :: o.value.get1(head_clause.terms[i]) == goal.evar_terms[i]
+    ensures head_clause.is_ground() && o.Some? ==> goal.emap_fully_resolved(emap) // o.value is empty map
+    ensures head_clause.is_ground() && o.Some? ==> goal.clause.make_fact(make_subst(emap, goal.subst)) == head_clause
+    // ensures o.Some? ==> goal.clause.make_fact(make_subst(emap,goal.subst)) == head_clause.make_fact(make_subst(emap,o.value))
     ensures emap.monotonically_increasing() // ensures forall e :: e in old(emap.evar_map) ==> e in emap.evar_map
+    // ensures forall v :: goal.subst.in1(v) && v.Var? && o.Some? ==> o.value.in1(v) && goal.subst.get1(v) == o.value.get1(v)
+    ensures o.Some? ==> forall i:nat | i < |head_clause.terms| ::
+                          (if head_clause.terms[i].Var? then o.value.get1(head_clause.terms[i]) == goal.evar_terms[i]
+                          else emap.evar_map[goal.evar_terms[i]].Some?)
+    // |goal.evar_terms| == |o.value.Values| // is this true?
 {
     // check if all terms in clause have correct mapping in goal.evar_terms
     var subst:EvarSubstitution := new_bijective_map<VarTerm, Evar>();
-    for i := 0 to |head_clause.terms| 
+    for i := 0 to |head_clause.terms|
         invariant emap.inv()
         invariant subst.valid()
         invariant goal.valid()
@@ -80,9 +100,12 @@ method unify(head_clause:Clause, goal:SearchClause, emap:EvarMap) returns (o:Opt
         invariant emap.monotonically_increasing() // invariant forall e :: e in old(emap.evar_map) ==> e in emap.evar_map
         invariant emap.is_more_resolved()
         invariant forall j :: (0 <= j < i && head_clause.terms[j].Var?) ==> subst.in1(head_clause.terms[j])
-        invariant forall j :: 0 <= j < i ==> head_clause.terms[j].Const? ==> emap.evar_map[goal.evar_terms[j]].Some?
+        invariant forall j:nat | j < i && head_clause.terms[j].Var? :: subst.get1(head_clause.terms[j]) == goal.evar_terms[j]
+        invariant forall j :: 0 <= j < i ==> head_clause.terms[j].Const? ==> emap.evar_map[goal.evar_terms[j]].Some? && Const(emap.evar_map[goal.evar_terms[j]].value) == head_clause.terms[j]
         invariant forall j :: i <= j < |head_clause.terms| ==> !subst.in1(head_clause.terms[j])
         invariant forall j :: i <= j < |goal.evar_terms| ==> !subst.in2(goal.evar_terms[j])
+        // invariant forall j:nat | j < i :: goal.subst.in1(goal.clause.terms[i]) && goal.clause.terms[i].Var? ==> subst.in1(goal.clause.terms[i]) && goal.subst.get1(goal.clause.terms[i]) == subst.get1(head_clause.terms[i])
+        // invariant head_clause.is_ground() ==> forall j:nat :: j < i ==> goal.clause.make_fact(make_subst(emap, goal.subst)).terms[j] == head_clause.terms[j]
     {
         if head_clause.terms[i].Var? {
             //print "a";
@@ -109,6 +132,9 @@ method unify(head_clause:Clause, goal:SearchClause, emap:EvarMap) returns (o:Opt
         }
     }
     reveal ToSet();
+    // assert(head_clause.is_ground() ==> forall i:nat :: i < |goal.clause.terms| ==> make_subst(emap, goal.subst)[goal.clause.terms[i]].c == emap.evar_map[goal.evar_terms[i]].value);
+    // assert(head_clause.is_ground() ==> forall i:nat :: i < |goal.clause.terms| ==> make_subst(emap, goal.subst)[goal.clause.terms[i]] == goal.clause.make_fact(make_subst(emap, goal.subst)).terms[i]);
+    // assert(head_clause.is_ground() ==> forall i:nat :: i < |goal.clause.terms| ==> goal.clause.make_fact(make_subst(emap, goal.subst)).terms[i] == head_clause.terms[i]);
     return Some(subst);
 }
 
@@ -125,12 +151,14 @@ method evarify(clause:Clause, subst:EvarSubstitution, emap:EvarMap)
     ensures  sc.valid()
     ensures  sc.valid_emap(emap)
     ensures  forall e :: subst'.in2(e) ==> e in emap.evar_map
+    ensures  forall e :: sc.subst.in2(e) ==> e in emap.evar_map
     ensures  emap.monotonically_increasing() // ensures forall e :: e in old(emap.evar_map) ==> e in emap.evar_map
     ensures  forall s :: subst.in1(s) ==> subst'.in1(s) && subst.get1(s) == subst'.get1(s)
     ensures  sc.clause == clause
     ensures  sc.clause.substitution_complete(make_subst(emap, subst'))
     // ensures  sc.subst.IsSubsetOf(subst') // sc.subst.Items() <= subst'.Items()
     ensures  forall v :: sc.subst.in1(v) && v.Var? ==> subst'.in1(v) && sc.subst.get1(v) == subst'.get1(v)
+    // ensures forall e :: e in subst'
 {
     subst' := subst;
     var local_subst:EvarSubstitution := new_bijective_map<VarTerm, Evar>();
@@ -156,6 +184,7 @@ method evarify(clause:Clause, subst:EvarSubstitution, emap:EvarMap)
         invariant reveal ToSet(); local_subst.Values() == ToSet(evar_terms)
         invariant forall j:nat | j < i :: local_subst.in1(clause.terms[j]) && (local_subst.get1(clause.terms[j]) == evar_terms[j])
         invariant forall v :: local_subst.in1(v) && v.Var? ==> subst'.in1(v) && local_subst.get1(v) == subst'.get1(v)
+        invariant forall j:nat | 0 <= j < i :: clause.terms[j].Const? ==> emap.evar_map[evar_terms[j]] == Some(clause.terms[j].c)
         // invariant forall e :: e in local_subst.l_to_r ==> e in subst'.l_to_r
     {
         var term := clause.terms[i];
@@ -168,7 +197,7 @@ method evarify(clause:Clause, subst:EvarSubstitution, emap:EvarMap)
                     // assert(!local_subst.in1(term));
                     // assert(!local_subst.in2(ev));
                     local_subst := local_subst.insert(term , ev);
-                } else if !subst'.in1(term) {
+                } else if !subst'.in1(term) { // TODO: THIS SHOULDN'T HAPPEN IF THE rule_restricted thing is there
                     var new_ev := emap.get_new_evar();
                     evar_terms := evar_terms + [new_ev];
                     // subst' := subst'[term := new_ev];
@@ -204,56 +233,36 @@ method search (rules:seq<Rule>, goal:SearchClause, emap:EvarMap, depth: nat) ret
     ensures emap.inv()
     ensures goal.valid_emap(emap) // TODO: Do we need to prove this at all times?
     ensures emap.monotonically_increasing() // ensures forall e :: e in old(emap.evar_map) ==> e in emap.evar_map
-    ensures b ==> proof.Some? && valid_proof(rules, goal.clause, proof.value)
-    ensures b ==> goal.emap_fully_resolved(emap)
-    ensures b ==> proof.Some? && Last(proof.value).new_fact() == goal.clause.make_fact(make_subst(emap, goal.subst))
+    // ensures b ==> goal.emap_fully_resolved(emap)
+    ensures b ==> goal.clause.substitution_concrete(make_subst(emap, goal.subst))
+    ensures b ==> proof.Some? && valid_proof(rules, goal.clause.make_fact(make_subst(emap, goal.subst)), proof.value)
+    // ensures b ==> proof.Some? && Last(proof.value).new_fact() == goal.clause.make_fact(make_subst(emap, goal.subst))
     // ensures emap.is_more_resolved'()
     decreases depth
-    // what the correct matching rule is (rule for which we returned true)
-    //   - maybe return a sequence of these rules
-    //   - build a 'substitution' map like Bryan using these rules
-    //       - a substitution is either a variable->evar or evar->const(resolve)
-    //   - ??
-    //   - reuse Bryan's spec
-    // ensures b ==> that rule works
-
-    // the different subst bi-maps are consistent // WRONG
-    // we should somehow say b==true ==> at no point we made the same evar resolve to two diff consts
-    // for each subst (at each instantiation of a rule down the tree), convert that subst into Bryan's substitution (using the 'global' evarmap)
-    //  -- keep a ghost state of seq<subst * rule> or a seq<applied_rules> * seq<subst for that rule>?
-    //  -- (var -> evar -> const) ==> (var -> const) like Bryan's substitution (a ground substitution)
-    //  -- do the above for ALL evars in our evarmap, the one for which search returns true (basically for all evars we want them to be present in substs)
-    //  --   at each proofstep, the number of evars for which the above stuff is not done decreases
-    // prove completeness of our substs? - we get a valid ProofStep for free?
 {
     if (depth == 0) {
         return false, None;
     }
     var current_emap:EvarMap := new EvarMap.Init(emap);
-    //print "Searching on ", goal, " with emap ", emap.evar_map, "\n";
     // find all rules that match current goal
     var matching_rules := find_matching_rules(rules, goal);
-    //print "\t matching_rules = ", matching_rules, "\n";
     assert(forall r :: r in matching_rules ==> valid_clause(r.head) && (forall c :: c in r.body ==> valid_clause(c)));
     // for all rules that match the current goal
     label AA: 
     for i := 0 to |matching_rules|
         invariant emap.inv()
         invariant current_emap.inv()
-        // invariant old@AA(current_emap.evar_map) == current_emap.evar_map
-        invariant unchanged@AA(current_emap)
+        invariant old@AA(current_emap.evar_map) == current_emap.evar_map
+        invariant old@AA(current_emap.next_evar) == current_emap.next_evar
+        // invariant unchanged@AA(current_emap)
         invariant forall j:nat | j < i :: valid_rule(matching_rules[j])
         // invariant goal.valid_emap(emap)
         invariant emap.monotonically_increasing() // invariant forall e :: e in old(emap.evar_map) ==> e in emap.evar_map
     {
         emap.copy(current_emap);
-        //print "\t i = ", i, "\n"; 
         var rule:Rule := matching_rules[i];
         assert(valid_clause(rule.head));
-        //print "\t matching_rule = ", rule, "\n";
         var option_subst := unify(rule.head, goal, emap);
-        
-        //print "\t option_subst = ", option_subst, "\n";
         
         var subst : EvarSubstitution;
         match option_subst {
@@ -264,15 +273,18 @@ method search (rules:seq<Rule>, goal:SearchClause, emap:EvarMap, depth: nat) ret
         var search_clauses:seq<SearchClause> := [];
         if |rule.body| == 0 {
             var concreteSubst := make_subst(emap, subst);
-            var proofStep := ProofStep(concreteSubst, rule, []);
+            var proofStep := ProofStep(map[], rule, []);
             assert rule in rules; // needed to use valid_program(rules) to conclude that valid_rule(rule) and then conclude that rule.head.is_ground() 
+            // assume (goal.clause.make_fact(make_subst(emap, goal.subst)) == rule.head.make_fact(concreteSubst));
             return true, Some([proofStep]);
         } else {
             for j := 0 to |rule.body|
                 invariant |search_clauses| == j
                 invariant emap.inv()
                 invariant current_emap.inv()
-                invariant unchanged@AA(current_emap)
+                // invariant unchanged@AA(current_emap)
+                invariant old@AA(current_emap.evar_map) == current_emap.evar_map
+                invariant old@AA(current_emap.next_evar) == current_emap.next_evar
                 invariant subst.valid()
                 // invariant current_emap.evar_map == old(current_emap.evar_map)
                 invariant forall sc :: sc in search_clauses ==> sc.valid()
@@ -284,6 +296,8 @@ method search (rules:seq<Rule>, goal:SearchClause, emap:EvarMap, depth: nat) ret
                 invariant forall i :: 0 <= i < j ==> search_clauses[i].clause.substitution_complete(make_subst(emap, subst))
                 invariant forall i :: 0 <= i < j ==> search_clauses[i].valid()
                 invariant valid_rule(rule)
+                // invariant forall v :: goal.subst.in1(v) && v.Var? ==> subst.in1(v) && goal.subst.get1(v) == subst.get1(v)
+                invariant forall ii :: 0 <= ii < |goal.clause.terms| && (rule.head.terms[ii].Var?) ==> subst.in1(rule.head.terms[ii]) && subst.get1(rule.head.terms[ii]) == goal.subst.get1(goal.clause.terms[ii])
                 invariant forall i :: 0 <= i < j ==> forall v :: search_clauses[i].subst.in1(v) && v.Var? ==> subst.in1(v) && search_clauses[i].subst.get1(v) == subst.get1(v)
                 // invariant forall k in old(subst) ==> k in subst
             {
@@ -295,26 +309,29 @@ method search (rules:seq<Rule>, goal:SearchClause, emap:EvarMap, depth: nat) ret
             var flag := true;
             ghost var proofs : seq<Proof> := [];
             assert forall i :: 0 <= i < |search_clauses| ==> search_clauses[i].clause.substitution_complete(make_subst(emap, subst));
-            for j := 0 to |search_clauses|
+            label L: for j := 0 to |search_clauses|
                 invariant emap.inv()
                 invariant current_emap.inv()
-                invariant unchanged@AA(current_emap)
+                // invariant unchanged@AA(current_emap)
+                invariant old@AA(current_emap.evar_map) == current_emap.evar_map
+                invariant old@AA(current_emap.next_evar) == current_emap.next_evar
                 invariant subst.valid()
                 invariant forall e :: subst.in2(e) ==> e in emap.evar_map
                 // invariant current_emap == old(current_emap)
                 invariant forall sc :: sc in search_clauses ==> sc.valid()
                 invariant forall sc :: sc in search_clauses ==> sc.valid_emap(emap)
                 // invariant forall e :: e in subst.Values ==> e in emap.evar_map
-                invariant emap.monotonically_increasing() // invariant forall e :: e in old(emap.evar_map) ==> e in emap.evar_map
+                invariant emap.monotonically_increasing@L() // invariant forall e :: e in old(emap.evar_map) ==> e in emap.evar_map
                 // invariant emap.is_more_resolved'()
-                invariant forall e :: e in old(emap.evar_map) ==> e in current_emap.evar_map // TODO: Make this a predicate inside evar.dfy
+                // invariant forall e :: e in old(emap.evar_map) ==> e in current_emap.evar_map // TODO: Make this a predicate inside evar.dfy
                 // invariant goal.valid_emap(emap)
                 // invariant flag ==> forall p :: p in proofs ==> p.Some?
                 invariant flag ==> (|proofs| == j)
                 invariant flag ==> (forall i :: 0 <= i < j ==> search_clauses[i].clause == rule.body[i])
-                invariant flag ==> (forall i :: 0 <= i < j ==> valid_proof(rules, search_clauses[i].clause, proofs[i]))
-                invariant flag ==> (forall k :: 0 <= k < j ==> search_clauses[k].emap_fully_resolved(emap))
                 invariant forall c :: c in search_clauses ==> forall e :: c.subst.in2(e) ==> e in emap.evar_map
+                invariant flag ==> (forall i :: 0 <= i < j ==> search_clauses[i].clause.substitution_concrete(make_subst(emap, search_clauses[i].subst)))
+                invariant flag ==> (forall i :: 0 <= i < j ==> valid_proof(rules, search_clauses[i].clause.make_fact(make_subst(emap, search_clauses[i].subst)), proofs[i]))
+                // invariant flag ==> (forall k :: 0 <= k < j ==> search_clauses[k].emap_fully_resolved(emap))
                 invariant flag ==> forall k :: 0 <= k < j ==> search_clauses[k].clause.make_fact(make_subst(emap, search_clauses[k].subst)) == Last(proofs[k]).new_fact();
                 invariant valid_rule(rule)
                 // invariant goal.emap_fully_resolved(emap) // not true as an invariant
@@ -327,30 +344,67 @@ method search (rules:seq<Rule>, goal:SearchClause, emap:EvarMap, depth: nat) ret
                     assert(proof_j.Some?);
                     proofs := proofs + [proof_j.value];
                 }
+                for k := 0 to j
+                    invariant forall kk :: 0 <= kk < k ==> search_clauses[kk].valid_emap(emap)
+                {
+                    search_clauses[k].monotonically_increasing_preserves_valid_emap@L(emap);
+                }
                 assert (forall k :: 0 <= k < j ==> search_clauses[k].emap_fully_resolved(emap));
             }
             if flag {
-                
+                /*
+                1. Use range restriction stuff to prove that emap_fully_resolved and substitution_concrete for the goal.clause
+                2. Use the fact that apply(subst, rule.head):seq<Evar> == apply(goal.subst, goal.clause):seq<Evar>
+                */
                 var concreteSubst := make_subst(emap, subst);
                 // assert |proofs| == |search_clauses| == |rule.body|;
-                assert forall i :: 0 <= i < |rule.body| ==> rule.body[i] == search_clauses[i].clause;
+                ////assert forall i :: 0 <= i < |rule.body| ==> rule.body[i] == search_clauses[i].clause;
                 // assert forall i :: 0 <= i < |rule.body| ==> search_clauses[i].valid_emap(emap);
                 // assume forall i :: 0 <= i < |rule.body| ==> search_clauses[i].emap_fully_resolved(emap); // TODO This will depend on some range restriction reasoning
-                assert forall i :: 0 <= i < |rule.body| ==> valid_proof(rules, search_clauses[i].clause, proofs[i]);
+                //// assert forall i :: 0 <= i < |rule.body| ==> valid_proof(rules, search_clauses[i].clause.make_fact(make_subst(emap, search_clauses[i].subst)), proofs[i]);
+                //// assert forall i :: 0 <= i < |rule.body| ==> valid_proof(rules, search_clauses[i].clause.make_fact(concreteSubst), proofs[i]);
                 // assert forall i :: 0 <= i < |rule.body| ==> valid_proof(rules, rule.body[i], proofs[i]);
-                assert forall i :: 0 <= i < |rule.body| ==> rule.body[i].make_fact(concreteSubst) == Last(proofs[i]).new_fact();
+                // assert forall i :: 0 <= i < |rule.body| ==> rule.body[i].make_fact(concreteSubst) == Last(proofs[i]).new_fact();
                 var proof := combine_proofs(rules, rule, concreteSubst, proofs);
+                assert(goal.subst.valid());
+                var goalSubst := make_subst(emap, goal.subst);
+                // assert();
+                // concreteSubst is concrete
+                // ==> forall vars in subst, subst[vars].Const?
+                // but subst[rule.head.terms[i]] == goal.subst[goal.clause.terms[i]] && |rule.head.terms| == |goal.clause.terms|
+                // and also |subst.Keys| == |goal.subst.Keys|
+                // therefore, all vars in goal.subst map to Consts
+                // assert forall e:VarTerm | subst.in1(e) :: emap.evar_map[subst.get1(e)].Some?;
+                // assert(forall e | e in goal.evar_terms :: e in subst.Values)
+                // assert goal.emap_fully_resolved(emap);
+                assert forall sc | sc in search_clauses :: forall v:VarTerm | v in sc.clause.terms :: concreteSubst[v].Const?;
+                assert forall e | e in goal.subst.Values() :: (exists sc | sc in search_clauses :: e in sc.subst.Values());
+                // var pp:set<VarTerm>;
+                // for k := 0 to |search_clauses| 
+                //     invariant pp == 
+                // {
+                //     pp := pp + (ToSet(search_clauses[i].clause.terms));
+                // }
+                // assert(forall v:VarTerm | v in rule.head.terms :: (exists c | c in rule.body :: v in c.terms));
+                assert(seq(|search_clauses|, i requires 0 <= i < |search_clauses| => search_clauses[i].clause) == rule.body);
+                // assert(forall v:VarTerm | v in rule.head.terms :: match_exists(v, rule.body));
+                // assert(forall v:VarTerm | v in goal.clause.terms :: match_exists(v, seq(|search_clauses|, i => search_clauses[i].clause)));
+
+                // assert(forall v:VarTerm | v in rule.head.terms :: (exists c | c in rule.body :: v in c.terms));
+                // assert ToSet(goal.clause.terms) <= (set x:Term | ((forall sc :: sc in search_clauses && x in sc.clause.terms) :: x));
+                // set x : T | P(x) :: x
+                // assert forall t:VarTerm | t in goal.clause.terms :: emap.evar_map[goal.subst.get1(t)].Some?;
+                assert goal.clause.substitution_concrete(goalSubst);
+                assert rule.head.make_fact(concreteSubst) == goal.clause.make_fact(goalSubst);
                 return true, Some(proof);
             }
         }
-        // assert(emap.monotonically_increasing());
         // emap.copy(current_emap);
-        // assert(emap.monotonically_increasing());
     }
     return false, None;
 }
 
-ghost method flatten_two_proofs(rules: seq<Rule>, subst: Substitution, goal1: Clause, proof1: Proof, goal2: Clause, proof2: Proof) returns (proof: Proof)
+ghost method flatten_two_proofs(rules: seq<Rule>, subst: Substitution, goal1: Fact, proof1: Proof, goal2: Fact, proof2: Proof) returns (proof: Proof)
     requires valid_proof(rules, goal1, proof1)
     requires valid_proof(rules, goal2, proof2)
     requires goal1.substitution_concrete(subst)
@@ -387,24 +441,25 @@ ghost method flatten_two_proofs(rules: seq<Rule>, subst: Substitution, goal1: Cl
 ghost method combine_proofs(rules: seq<Rule>, rule: Rule, subst: Substitution, proofs: seq<Proof>) returns (proof: Proof)
     requires |rule.body| == |proofs| >= 1
     requires rule in rules
-    requires forall i :: 0 <= i < |rule.body| ==> valid_proof(rules, rule.body[i], proofs[i])
     requires rule.head.substitution_concrete(subst)
-    requires forall i :: 0 <= i < |rule.body| ==> rule.body[i].substitution_concrete(subst) && rule.body[i].make_fact(subst) == Last(proofs[i]).new_fact();
-    ensures  valid_proof(rules, rule.head, proof)
+    requires forall i :: 0 <= i < |rule.body| ==> rule.body[i].substitution_concrete(subst) 
+    requires forall i :: 0 <= i < |rule.body| ==> valid_proof(rules, rule.body[i].make_fact(subst), proofs[i])
+    requires forall i :: 0 <= i < |rule.body| ==> rule.body[i].make_fact(subst) == Last(proofs[i]).new_fact()
+    ensures  valid_proof(rules, rule.head.make_fact(subst), proof)
 {
     proof := proofs[0];
-    var goal := rule.body[0];
+    var goal := rule.body[0].make_fact(subst);
     for i := 1 to |proofs|
         invariant valid_proof(rules, goal, proof)
         invariant goal.substitution_concrete(subst)
         invariant goal.make_fact(subst) == Last(proof).new_fact()
-        invariant goal == rule.body[i-1]
+        invariant goal == rule.body[i-1].make_fact(subst)
         invariant forall j :: 0 <= j < |proof| ==> proof[j].valid()
         invariant forall j :: 0 <= j < i - 1 ==> rule.body[j].make_fact(subst) in Last(proof).facts
     {
-        var new_proof := flatten_two_proofs(rules, subst, rule.body[i], proofs[i], goal, proof);
+        var new_proof := flatten_two_proofs(rules, subst, rule.body[i].make_fact(subst), proofs[i], goal, proof);
         proof := new_proof;
-        goal := rule.body[i];
+        goal := rule.body[i].make_fact(subst);
     }
     var last_step := ProofStep(subst, rule, Last(proof).facts + [ Last(proof).new_fact() ]);
     proof := proof + [last_step];
