dafny/top-down/search_clause.dfy
@@ -31,6 +31,7 @@ datatype SearchClause = SearchClause(name:string, evar_terms:seq<Evar>, clause: 
     {
         && (forall e:Evar :: e in evar_terms ==> e in emap.evar_map)
         && (forall e:Evar :: subst.in2(e) ==> e in emap.evar_map)
+        && (forall i:nat | i < |clause.terms| :: clause.terms[i].Const? ==> emap.evar_map[evar_terms[i]] == Some(clause.terms[i].c))
         // && (forall e:Evar :: e in subst.Values ==> e in emap.evar_map)
         // multiset(evar_terms) <= multiset(emap.evar_map.Keys)
     }
@@ -41,6 +42,51 @@ datatype SearchClause = SearchClause(name:string, evar_terms:seq<Evar>, clause: 
         requires valid_emap(emap)
     {
         forall e:Evar :: e in evar_terms ==> emap.evar_map[e].Some?
+    }
+
+    lemma make_fact_preserves(emap: EvarMap)
+        requires valid()
+        requires emap.inv()
+        requires subst.valid()
+        requires valid_emap(emap)
+        requires emap_fully_resolved(emap)
+        requires forall e:Evar :: subst.in2(e) ==> e in emap.evar_map
+        requires clause.substitution_concrete(make_subst(emap, subst))
+        ensures forall i:nat | i < |clause.make_fact(make_subst(emap, subst)).terms| 
+                       :: clause.make_fact(make_subst(emap, subst)).terms[i].c == emap.evar_map[evar_terms[i]].value
+    {
+        var s := make_subst(emap, subst);
+        var f := clause.make_fact(s);
+        assert |f.terms| == |evar_terms|;
+        for i := 0 to |f.terms|
+            invariant forall j:nat | j < i :: f.terms[j].Const?
+            invariant forall j:nat | j < i :: emap.evar_map[evar_terms[j]].Some?
+            // invariant forall j:nat | j < i :: evar_terms[j] in emap.evar_map
+            invariant forall j:nat | j < i :: f.terms[j].c == emap.evar_map[evar_terms[j]].value
+        {
+            var lhs := f.terms[i];
+            assert (lhs.Const?);
+            var rhs := emap.evar_map[evar_terms[i]];
+            assert (rhs.Some?);
+            assert (subst.get1(clause.terms[i]) == evar_terms[i]);
+            assert (s[clause.terms[i]] == Const(rhs.value));
+            if (s[clause.terms[i]].Var?) {
+                assert (s[clause.terms[i]] == f.terms[i]);
+                assert (lhs.c == rhs.value);
+            }
+            // assert (evar_terms[i] == subst.)
+            assert (lhs.c == rhs.value);
+        } 
+    }
+
+    twostate lemma monotonically_increasing_preserves_valid_emap(emap: EvarMap)
+        requires old(emap.inv())
+        requires valid()
+        requires old(valid_emap(emap))
+        requires emap.monotonically_increasing()
+        ensures valid_emap(emap)
+    {
+
     }
 
 /*
